SStructTT/SStruct/Erasure/Step.lean
@@ -19,85 +19,83 @@ inductive Value : Tm Srt -> Prop where
   | null : Value .null
 
 @[scoped aesop safe [constructors]]
-inductive Drop : Tm Srt -> Tm Srt -> Prop where
+inductive Step0 : Tm Srt -> Tm Srt -> Prop where
   | app_M {m m'} n :
-    Drop m m' ->
-    Drop (.app m n) (.app m' n)
+    Step0 m m' ->
+    Step0 (.app m n) (.app m' n)
   | app_N m {n n'} :
-    Drop n n' ->
-    Drop (.app m n) (.app m n')
+    Step0 n n' ->
+    Step0 (.app m n) (.app m n')
   | tup_M {m m'} n s :
-    Drop m m' ->
-    Drop (.tup m n s) (.tup m' n s)
+    Step0 m m' ->
+    Step0 (.tup m n s) (.tup m' n s)
   | tup_N m {n n'} s :
-    Drop n n' ->
-    Drop (.tup m n s) (.tup m n' s)
+    Step0 n n' ->
+    Step0 (.tup m n s) (.tup m n' s)
   | prj_M {m m'} n :
-    Drop m m' ->
-    Drop (.prj m n) (.prj m' n)
+    Step0 m m' ->
+    Step0 (.prj m n) (.prj m' n)
   | ite_M {m m'} n1 n2 :
-    Drop m m' ->
-    Drop (.ite m n1 n2) (.ite m' n1 n2)
+    Step0 m m' ->
+    Step0 (.ite m n1 n2) (.ite m' n1 n2)
   | drop_elim m n :
-    Drop (.drop m n) n
+    Step0 (.drop m n) n
 
 @[scoped aesop safe [constructors]]
-inductive CoreStep : Tm Srt -> Tm Srt -> Prop where
+inductive Step1 : Tm Srt -> Tm Srt -> Prop where
   | app_M {m m'} n :
-    CoreStep m m' ->
-    CoreStep (.app m n) (.app m' n)
+    Step1 m m' ->
+    Step1 (.app m n) (.app m' n)
   | app_N m {n n'} :
-    CoreStep n n' ->
-    CoreStep (.app m n) (.app m n')
+    Step1 n n' ->
+    Step1 (.app m n) (.app m n')
   | beta m n s :
     Value n ->
-    CoreStep (.app (.lam m s) n) m.[n/]
+    Step1 (.app (.lam m s) n) m.[n/]
   | tup_M {m m'} n s :
-    CoreStep m m' ->
-    CoreStep (.tup m n s) (.tup m' n s)
+    Step1 m m' ->
+    Step1 (.tup m n s) (.tup m' n s)
   | tup_N m {n n'} s :
-    CoreStep n n' ->
-    CoreStep (.tup m n s) (.tup m n' s)
+    Step1 n n' ->
+    Step1 (.tup m n s) (.tup m n' s)
   | prj_M {m m'} n :
-    CoreStep m m' ->
-    CoreStep (.prj m n) (.prj m' n)
+    Step1 m m' ->
+    Step1 (.prj m n) (.prj m' n)
   | prj_elim {m1 m2} n {s} :
     Value (.tup m1 m2 s) ->
-    CoreStep (.prj (.tup m1 m2 s) n) n.[m2,m1/]
+    Step1 (.prj (.tup m1 m2 s) n) n.[m2,m1/]
   | ite_M {m m'} n1 n2 :
-    CoreStep m m' ->
-    CoreStep (.ite m n1 n2) (.ite m' n1 n2)
+    Step1 m m' ->
+    Step1 (.ite m n1 n2) (.ite m' n1 n2)
   | ite_tt n1 n2 :
-    CoreStep (.ite .tt n1 n2) n1
+    Step1 (.ite .tt n1 n2) n1
   | ite_ff n1 n2 :
-    CoreStep (.ite .ff n1 n2) n2
-  | rw_elim m :
-    CoreStep (.rw m) m
+    Step1 (.ite .ff n1 n2) n2
 
-abbrev Drops (m m' : Tm Srt) : Prop := Star Drop m m'
+abbrev Red0 (m m' : Tm Srt) : Prop := Star Step0 m m'
 
 inductive Step (m : Tm Srt) : Tm Srt -> Prop where
-  | intro {m' n} : Drops m m' -> CoreStep m' n -> Step m n
+  | intro {m' n} : Red0 m m' -> Step1 m' n -> Step m n
 
 notation:50 m:50 " ~>> " n:50 => Step m n
 notation:50 m:50 " ~>>* " n:50 => ARS.Star Step m n
 
-lemma Drops.var_inv {x} {t : Tm Srt} :
-    Drops (.var x) t -> t = .var x := by
+lemma Red0.var_inv {x} {t : Tm Srt} :
+    Red0 (.var x) t -> t = .var x := by
   intro rd; induction rd
   case R => simp
   case SE st ih =>
     subst_vars; cases st
 
-lemma Drops.lam_inv {m t : Tm Srt} {s} :
-    Drops (.lam m s) t -> t = .lam m s := by
+lemma Red0.lam_inv {m t : Tm Srt} {s} :
+    Red0 (.lam m s) t -> t = .lam m s := by
   intro rd; induction rd
   case R => simp
   case SE st e => subst_vars; cases st
 
-lemma Drops.app_inv {m n t : Tm Srt} :
-    Drops (.app m n) t ->
-    ∃ m' n', t = .app m' n' ∧ Drops m m' ∧ Drops n n' := by
+lemma Red0.app_inv {m n t : Tm Srt} :
+    Red0 (.app m n) t ->
+    ∃ m' n', t = .app m' n' ∧ Red0 m m' ∧ Red0 n n' := by
   intro rd; induction rd
   case R =>
     exists m, n; aesop
@@ -114,9 +112,9 @@ lemma Drops.app_inv {m n t : Tm Srt} :
       . assumption
       . apply Star.SE rd2 st
 
-lemma Drops.tup_inv {m n t : Tm Srt} {s} :
-    Drops (.tup m n s) t ->
-    ∃ m' n', t = .tup m' n' s ∧ Drops m m' ∧ Drops n n' := by
+lemma Red0.tup_inv {m n t : Tm Srt} {s} :
+    Red0 (.tup m n s) t ->
+    ∃ m' n', t = .tup m' n' s ∧ Red0 m m' ∧ Red0 n n' := by
   intro rd; induction rd
   case R => exists m, n; aesop
   case SE st ih =>
@@ -132,9 +130,9 @@ lemma Drops.tup_inv {m n t : Tm Srt} {s} :
       . assumption
       . apply Star.SE rd2 st
 
-lemma Drops.prj_inv {m n t : Tm Srt} :
-    Drops (.prj m n) t ->
-    ∃ m', t = .prj m' n ∧ Drops m m' := by
+lemma Red0.prj_inv {m n t : Tm Srt} :
+    Red0 (.prj m n) t ->
+    ∃ m', t = .prj m' n ∧ Red0 m m' := by
   intro rd; induction rd
   case R => exists m; aesop
   case SE st ih =>
@@ -145,19 +143,19 @@ lemma Drops.prj_inv {m n t : Tm Srt} :
       exists mx; simp
       apply Star.SE rd st
 
-lemma Drops.tt_inv {t : Tm Srt} : Drops .tt t -> t = .tt := by
+lemma Red0.tt_inv {t : Tm Srt} : Red0 .tt t -> t = .tt := by
   intro rd; induction rd
   case R => simp
   case SE st ih => subst_vars; cases st
 
-lemma Drops.ff_inv {t : Tm Srt} : Drops .ff t -> t = .ff := by
+lemma Red0.ff_inv {t : Tm Srt} : Red0 .ff t -> t = .ff := by
   intro rd; induction rd
   case R => simp
   case SE st ih => subst_vars; cases st
 
-lemma Drops.ite_inv {m n1 n2 t : Tm Srt} :
-    Drops (.ite m n1 n2) t ->
-    ∃ m', t = .ite m' n1 n2 ∧ Drops m m' := by
+lemma Red0.ite_inv {m n1 n2 t : Tm Srt} :
+    Red0 (.ite m n1 n2) t ->
+    ∃ m', t = .ite m' n1 n2 ∧ Red0 m m' := by
   intro rd; induction rd
   case R => exists m; aesop
   case SE st ih =>
@@ -168,13 +166,8 @@ lemma Drops.ite_inv {m n1 n2 t : Tm Srt} :
       exists mx; simp
       apply Star.SE rd st
 
-lemma Drops.rw_inv {m t : Tm Srt} : Drops (.rw m) t -> t = .rw m := by
-  intro rd; induction rd
-  case R => simp
-  case SE st ih => subst_vars; cases st
-
-lemma Drops.drop_inv {m n a b : Tm Srt} :
-    Drops (.drop m n) a -> Drop a b -> Drops n b := by
+lemma Red0.drop_inv {m n a b : Tm Srt} :
+    Red0 (.drop m n) a -> Step0 a b -> Red0 n b := by
   intro rd st; induction rd generalizing b
   case R =>
     cases st
@@ -185,40 +178,40 @@ lemma Drops.drop_inv {m n a b : Tm Srt} :
       assumption
     . assumption
 
-lemma Drops.ptr_inv {l} {t : Tm Srt} :
-    Drops (.ptr l) t -> t = .ptr l := by
+lemma Red0.ptr_inv {l} {t : Tm Srt} :
+    Red0 (.ptr l) t -> t = .ptr l := by
   intro rd; induction rd
   case R => simp
   case SE st ih =>
     subst_vars; cases st
 
-lemma Drops.null_inv {t : Tm Srt} :
-    Drops .null t -> t = .null := by
+lemma Red0.null_inv {t : Tm Srt} :
+    Red0 .null t -> t = .null := by
   intro rd; induction rd
   case R => simp
   case SE st ih =>
     subst_vars; cases st
 
-lemma Drops.app {m m' n n' : Tm Srt} :
-    Drops m m' -> Drops n n' -> Drops (.app m n) (.app m' n') := by
+lemma Red0.app {m m' n n' : Tm Srt} :
+    Red0 m m' -> Red0 n n' -> Red0 (.app m n) (.app m' n') := by
   intro rm rn
   apply (@Star.trans _ _ (.app m' n))
   apply Star.hom _ _ rm; aesop
   apply Star.hom _ _ rn; aesop
 
-lemma Drops.tup {m m' n n' : Tm Srt} {s} :
-    Drops m m' -> Drops n n' -> Drops (.tup m n s) (.tup m' n' s) := by
+lemma Red0.tup {m m' n n' : Tm Srt} {s} :
+    Red0 m m' -> Red0 n n' -> Red0 (.tup m n s) (.tup m' n' s) := by
   intro rm rn
   apply (@Star.trans _ _ (.tup m' n s))
   apply Star.hom _ _ rm; aesop
   apply Star.hom _ _ rn; aesop
 
-lemma Drops.prj {m m' n : Tm Srt} :
-    Drops m m' -> Drops (.prj m n) (.prj m' n) := by
+lemma Red0.prj {m m' n : Tm Srt} :
+    Red0 m m' -> Red0 (.prj m n) (.prj m' n) := by
   intro rm; apply Star.hom _ _ rm; aesop
 
-lemma Drops.ite {m m' n1 n2 : Tm Srt} :
-    Drops m m' -> Drops (.ite m n1 n2) (.ite m' n1 n2) := by
+lemma Red0.ite {m m' n1 n2 : Tm Srt} :
+    Red0 m m' -> Red0 (.ite m n1 n2) (.ite m' n1 n2) := by
   intro rm; apply Star.hom _ _ rm; aesop
 
 lemma Step.app_M {m m' n : Tm Srt} :
@@ -226,7 +219,7 @@ lemma Step.app_M {m m' n : Tm Srt} :
   intro st
   rcases st with ⟨rd, st⟩
   constructor
-  . apply Drops.app rd Star.R
+  . apply Red0.app rd Star.R
   . constructor; assumption
 
 lemma Step.app_N {m n n' : Tm Srt} :
@@ -234,7 +227,7 @@ lemma Step.app_N {m n n' : Tm Srt} :
   intro st
   rcases st with ⟨rd, st⟩
   constructor
-  . apply Drops.app Star.R rd
+  . apply Red0.app Star.R rd
   . constructor; assumption
 
 lemma Step.tup_M {m m' n : Tm Srt} {s} :
@@ -242,7 +235,7 @@ lemma Step.tup_M {m m' n : Tm Srt} {s} :
   intro st
   rcases st with ⟨rd, st⟩
   constructor
-  . apply Drops.tup rd Star.R
+  . apply Red0.tup rd Star.R
   . constructor; assumption
 
 lemma Step.tup_N {m n n' : Tm Srt} {s} :
@@ -250,7 +243,7 @@ lemma Step.tup_N {m n n' : Tm Srt} {s} :
   intro st
   rcases st with ⟨rd, st⟩
   constructor
-  . apply Drops.tup Star.R rd
+  . apply Red0.tup Star.R rd
   . constructor; assumption
 
 lemma Step.prj_M {m m' n : Tm Srt} :
@@ -258,7 +251,7 @@ lemma Step.prj_M {m m' n : Tm Srt} :
   intro st
   rcases st with ⟨rd, st⟩
   constructor
-  . apply Drops.prj rd
+  . apply Red0.prj rd
   . constructor; assumption
 
 lemma Step.ite_M {m m' n1 n2 : Tm Srt} :
@@ -266,7 +259,7 @@ lemma Step.ite_M {m m' n1 n2 : Tm Srt} :
   intro st
   rcases st with ⟨rd, st⟩
   constructor
-  . apply Drops.ite rd
+  . apply Red0.ite rd
   . constructor; assumption
 
 lemma Step.drop {m n n' : Tm Srt} :
