SStructTT/SStruct/Erasure/Progress.lean
@@ -7,54 +7,65 @@ variable {Srt : Type} [ord : SrtOrder Srt]
 
 lemma Erased.pi_canonical {A B C m : SStruct.Tm Srt} {m' r s} :
     [] ;; [] ⊢ m ▷ m' : C -> C === .pi A B r s -> Value m' ->
-    ∃ A n n', m = .lam A n r s ∧ m' = .lam n' s := by
+    ∃ n', m' = .lam n' s := by
   generalize e1: [] = Γ
   generalize e2: [] = Δ
   intro ty eq vl; induction ty <;> try trivial
   all_goals try false_conv
   case lam_im A B m m' _ _ _ _ _ _ _  =>
     have ⟨_, _, eqA, eqB⟩ := Static.Conv.pi_inj eq
-    subst_vars; exists A, m, m'
+    subst_vars; exists m'
   case lam_ex A B m m' _ _ _ _ _ _ _ =>
     have ⟨_, _, eqA, eqB⟩ := Static.Conv.pi_inj eq
-    subst_vars; exists A, m, m'
+    subst_vars; exists m'
+  case rw tyA erm tyn ih =>
+    subst_vars; simp_all
+    have ⟨eq, ty⟩ := tyn.closed_idn tyA
+    apply ih; apply Conv.trans eq; assumption
   case conv ih =>
     apply ih <;> try assumption
     apply Conv.trans <;> assumption
 
 lemma Erased.sig_canonical {A B C m : SStruct.Tm Srt} {m' r s} :
     [] ;; [] ⊢ m ▷ m' : C -> C === .sig A B r s -> Value m' ->
-    ∃ m1 m1' m2 m2', m = .tup m1 m2 r s ∧ m' = .tup m1' m2' s  := by
+    ∃ m1' m2', m' = .tup m1' m2' s  := by
   generalize e1: [] = Γ
   generalize e2: [] = Δ
   intro ty eq vl; induction ty <;> try trivial
   all_goals try false_conv
   case tup_im A0 B0 m m' n _ _ _ _ _ _ =>
     have ⟨_, _, _, _⟩ := Static.Conv.sig_inj eq
-    subst_vars; exists m, m', n, .null
+    subst_vars; exists m', .null
   case tup_ex A0 B0 m m' n n' _ _ _ _ _ _ _ _ =>
     have ⟨_, _, _, _⟩ := Static.Conv.sig_inj eq
-    subst_vars; exists m, m', n, n'
+    subst_vars; exists m', n'
+  case rw tyA erm tyn ih =>
+    subst_vars; simp_all
+    have ⟨eq, ty⟩ := tyn.closed_idn tyA
+    apply ih; apply Conv.trans eq; assumption
   case conv ihm =>
     apply ihm <;> try assumption
     apply Conv.trans <;> assumption
 
 lemma Erased.bool_canonical {C m : SStruct.Tm Srt} {m'} :
-    [] ;; [] ⊢ m ▷ m' : C -> C === .bool -> Value m' ->
-      (m = .tt ∧ m' = .tt) ∨ (m = .ff ∧ m' = .ff) := by
+    [] ;; [] ⊢ m ▷ m' : C -> C === .bool -> Value m' -> m' = .tt ∨ m' = .ff := by
   generalize e1: [] = Γ
   generalize e2: [] = Γ
   intro ty eq vl; induction ty <;> try trivial
   all_goals try false_conv
   case tt => simp
   case ff => simp
+  case rw tyA erm tyn ih =>
+    subst_vars; simp_all
+    have ⟨eq, ty⟩ := tyn.closed_idn tyA
+    apply ih; apply Conv.trans eq; assumption
   case conv ihm =>
     apply ihm <;> try assumption
     apply Conv.trans <;> assumption
 
 theorem Erased.progress {A m} {m' : Tm Srt} :
     [] ;; [] ⊢ m ▷ m' : A ->
-      (∃ n', m' ~>> n') ∨ (∃ v, Drops m' v ∧ Value v) := by
+      (∃ n', m' ~>> n') ∨ (∃ v, Red0 m' v ∧ Value v) := by
   generalize e1: [] = Γ
   generalize e2: [] = Δ
   intro er; induction er <;> (subst_vars; try trivial)
@@ -73,11 +84,11 @@ theorem Erased.progress {A m} {m' : Tm Srt} :
       left; exists Tm.app m' .null
       apply Step.app_M; assumption
     | .inr ⟨v, rd, vl⟩ =>
-      replace erm := erm.preserve_drops rd
-      have ⟨_, m, m', e1, e2⟩ := erm.pi_canonical Conv.R vl
+      replace erm := erm.preservation0' rd
+      have ⟨m', e⟩ := erm.pi_canonical Conv.R vl
       subst_vars; left; exists m'.[.null/]
       constructor
-      . apply Drops.app rd Star.R
+      . apply Red0.app rd Star.R
       . aesop
   case app_ex m m' n n' _ erm ern ihm ihn mrg =>
     cases mrg; simp_all
@@ -86,17 +97,17 @@ theorem Erased.progress {A m} {m' : Tm Srt} :
       left; exists Tm.app m' n'
       apply Step.app_M; assumption
     | .inr ⟨v1, rd1, vl1⟩ =>
-      replace erm := erm.preserve_drops rd1
+      replace erm := erm.preservation0' rd1
       match ihn with
       | .inl ⟨n', _⟩ =>
         left; exists Tm.app m' n'
         apply Step.app_N; assumption
       | .inr ⟨v2, rd2, vl2⟩ =>
-        replace ern := ern.preserve_drops rd2
-        have ⟨_, m, m', e1, e2⟩ := erm.pi_canonical Conv.R vl1
+        replace ern := ern.preservation0' rd2
+        have ⟨m', e⟩ := erm.pi_canonical Conv.R vl1
         subst_vars; left; exists m'.[v2/]
         constructor
-        . apply Drops.app rd1 rd2
+        . apply Red0.app rd1 rd2
         . aesop
   case tup_im m m' n s _ _ _ _ ih =>
     simp_all
@@ -106,7 +117,7 @@ theorem Erased.progress {A m} {m' : Tm Srt} :
       apply Step.tup_M; assumption
     | .inr ⟨v, rd, vl⟩ =>
       right; exists .tup v .null s; and_intros
-      . apply Drops.tup rd Star.R
+      . apply Red0.tup rd Star.R
       . aesop
   case tup_ex m m' n n' s _ _ _ _ ihm ihn mrg =>
     cases mrg; simp_all
@@ -121,7 +132,7 @@ theorem Erased.progress {A m} {m' : Tm Srt} :
         apply Step.tup_N; assumption
       | .inr ⟨v2, rd2, vl2⟩ =>
         right; exists .tup v1 v2 s; and_intros
-        . apply Drops.tup rd1 rd2
+        . apply Red0.tup rd1 rd2
         . aesop
   case prj_im C m m' n n' _ _ _ _ _ _ erm _ ihm _ mrg =>
     cases mrg; simp_all
@@ -130,11 +141,11 @@ theorem Erased.progress {A m} {m' : Tm Srt} :
       left; exists Tm.prj m n'
       apply Step.prj_M; assumption
     | .inr ⟨v, rd, vl⟩ =>
-      replace erm := erm.preserve_drops rd
-      have ⟨m1, m1', m2, m2', _, _⟩ := erm.sig_canonical Conv.R vl
+      replace erm := erm.preservation0' rd
+      have ⟨m1', m2', _⟩ := erm.sig_canonical Conv.R vl
       subst_vars; left; exists n'.[m2',m1'/]
       constructor
-      . apply Drops.prj rd
+      . apply Red0.prj rd
       . aesop
   case prj_ex C m m' n n' _ _ _ _ _ _ erm _ ihm _ mrg =>
     cases mrg; simp_all
@@ -143,11 +154,11 @@ theorem Erased.progress {A m} {m' : Tm Srt} :
       left; exists Tm.prj m n'
       apply Step.prj_M; assumption
     | .inr ⟨v, rd, vl⟩ =>
-      replace erm := erm.preserve_drops rd
-      have ⟨m1, m1', m2, m2', _, _⟩ := erm.sig_canonical Conv.R vl
+      replace erm := erm.preservation0' rd
+      have ⟨m1', m2', _⟩ := erm.sig_canonical Conv.R vl
       subst_vars; left; exists n'.[m2',m1'/]
       constructor
-      . apply Drops.prj rd
+      . apply Red0.prj rd
       . aesop
   case tt => right; exists .tt; aesop
   case ff => right; exists .ff; aesop
@@ -158,15 +169,15 @@ theorem Erased.progress {A m} {m' : Tm Srt} :
       left; exists Tm.ite m' n1' n2'
       apply Step.ite_M; assumption
     | .inr ⟨v, rd, vl⟩ =>
-      replace erm := erm.preserve_drops rd
-      match erm.bool_canonical Conv.R vl with
-      | .inl ⟨e1, e2⟩ =>
+      replace erm := erm.preservation0' rd
+      cases erm.bool_canonical Conv.R vl with
+      | inl =>
         subst_vars; left; exists n1'; constructor
-        . apply Drops.ite rd
+        . apply Red0.ite rd
         . constructor
-      | .inr ⟨e1, e2⟩ =>
+      | inr =>
         subst_vars; left; exists n2'; constructor
-        . apply Drops.ite rd
+        . apply Red0.ite rd
         . constructor
   case drop s lw h erm ern ihm ihn mrg =>
     cases mrg; simp_all
@@ -180,8 +191,5 @@ theorem Erased.progress {A m} {m' : Tm Srt} :
         constructor
         assumption
       . assumption
-  case rw m n _ _ _ _ _ _ _ _ =>
-    left; exists m; constructor
-    . apply Star.R
-    . constructor
-  case conv ih => aesop
+  case rw => aesop
+  case conv => aesop
